update Chap10 Sec06 Termination of Insertion sort

Fpil/Chap10/Sec06.lean
@@ -1,1 +1,73 @@
 /- # Insertion Sort and Array Mutation -/
+
+#check dbgTraceIfShared
+
+-- # The Inner Loop
+
+def insertSorted [Ord α] (arr : Array α) (i : Fin arr.size) : Array α :=
+  match i with
+  | ⟨0, _⟩ => arr
+  | ⟨i' + 1, _⟩ =>
+    have : i' < arr.size := by
+      simp [Nat.lt_of_succ_lt, *]
+    match Ord.compare arr[i'] arr[i] with
+    | .lt | .eq => arr
+    | .gt =>
+      insertSorted (arr.swap ⟨i', by assumption⟩ i) ⟨i', by simp [*]⟩
+
+#check Nat.lt_of_succ_lt
+
+-- # The Outer Loop
+
+-- partial def insertionSortLoop [Ord α] (arr : Array α) (i : Nat) : Array α :=
+--   if h : i < arr.size then
+--     insertionSortLoop (insertSorted arr ⟨i, h⟩) (i + 1)
+--   else
+--     arr
+
+-- #eval insertionSortLoop #[3, 1, 4, 1, 5, 9, 2, 6] 0
+
+-- #eval insertionSortLoop #["metamorphic", "igneous", "sedentary"] 0
+
+-- ## Termination
+
+-- theorem insert_sorted_size_eq [Ord α] (arr : Array α) (i : Fin arr.size) :
+--   (insertSorted arr i).size == arr.size := by
+--   match i with
+--   | ⟨j, isLt⟩ =>
+--     induction j with
+--     | zero => simp [insertSorted]
+--     | succ j' ih =>
+--       simp [insertSorted]
+--       split <;> try rfl
+
+theorem insert_sorted_size_eq [Ord α] (len : Nat) (i : Nat) :
+  (arr : Array α) → (isLt : i < arr.size) → arr.size = len →
+  (insertSorted arr ⟨i, isLt⟩).size = len := by
+  induction i with
+  | zero =>
+    intro arr isLt hLen
+    simp [insertSorted, hLen]
+  | succ i' ih =>
+    intro arr isLt hLen
+    simp [insertSorted]
+    split <;> try simp[*]
+
+
+def insertionSortLoop [Ord α] (arr : Array α) (i : Nat) : Array α :=
+  if h : i < arr.size then
+    have : Array.size (insertSorted arr ⟨i, h⟩) - (i + 1) < Array.size arr - i := by
+      rw [insert_sorted_size_eq arr.size i arr h rfl]
+      simp [Nat.sub_succ_lt_self, *]
+    insertionSortLoop (insertSorted arr ⟨i, h⟩) (i + 1)
+  else
+    arr
+  termination_by insertionSortLoop arr i => arr.size - i
+
+-- # The Driver Function
+
+def insertionSort [Ord α] (arr : Array α) : Array α :=
+  insertionSortLoop arr 0
+
+#eval insertionSort #[3, 1, 7, 4]
+#eval insertionSort #[ "quartz", "marble", "granite", "hematite"]
